Prove more hol4-base assumptions
There are now 13 left, and they all appear to require changes to the
setup. Some are to do with constants that are more specified in HOL than
OT (such as PRE and arithmetic$-). The rest are mostly to do with
boolTheory, which has not been recorded, and includes things like
TYPE_DEFINITION.

src/boss/prove_base_assumsScript.sml
@@ -1,4 +1,4 @@
-open HolKernel boolLib Opentheory lcsymtacs
+open HolKernel boolLib Opentheory lcsymtacs BasicProvers
 
 val Thy = "prove_base_assums";
 
@@ -163,7 +163,22 @@ val EQF_INTRO = SYM o (CONV_RULE(REWR_CONV(GSYM F_iff)))
 val not_and = hd (amatch ``¬(t1 ∧ t2) ⇔ _``)
 val not_not = hd (amatch ``¬(¬ _)``)
 val disj_comm = hd (amatch ``_ ∨ _ ⇔ _ ∨ _``)
-val th1 = store_thm("th1", el 1 goals |> concl, PURE_REWRITE_TAC[not_and,not_not,Once disj_comm,bool_cases])
+
+val T_or = hd(amatch``T ∨ t``)
+val or_T = hd(amatch``t ∨ T``)
+val F_or = hd(amatch``F ∨ t``)
+val or_F = hd(amatch``t ∨ F``)
+val or_i = hd(amatch``t ∨ t``)
+
+val truth = hd(amatch``T``);
+val not_F = hd(amatch``¬F``)
+
+val bool_cases = hd(amatch``(x = T) ∨ _``)
+
+val th1 = store_thm("th1", el 1 goals |> concl,
+  PURE_REWRITE_TAC[not_and,not_not]
+  \\ Q.SPEC_THEN`t`FULL_STRUCT_CASES_TAC bool_cases
+  \\ PURE_REWRITE_TAC[or_T,or_F,not_F])
 
 (* 2, 3, 4 are TYPE_DEFINITION *)
 
@@ -182,7 +197,7 @@ val th5 = store_thm("th5", el 5 goals |> concl,
   \\ rpt gen_tac \\ strip_tac
   \\ PURE_REWRITE_TAC[GSYM fun_eq_thm]
   \\ ho_match_mp_tac list_ind
-  \\ rpt BasicProvers.VAR_EQ_TAC
+  \\ rpt VAR_EQ_TAC
   \\ conj_tac >- (first_assum MATCH_ACCEPT_TAC)
   \\ rpt strip_tac
   \\ rpt (last_x_assum(qspecl_then[`h`,`x`]mp_tac))
@@ -216,13 +231,8 @@ val th6 = store_thm("th6", el 6 goals |> concl,
   \\ rpt(first_x_assum(qspec_then`b`SUBST_ALL_TAC))
   \\ REFL_TAC)
 
-val bool_cases = hd(amatch``(x = T) ∨ _``)
-
 val if_T = hd(amatch``(if T then _ else _) = _``)
 val if_F = hd(amatch``(if F then _ else _) = _``)
-
-val truth = hd(amatch``T``);
-val not_F = hd(amatch``¬F``)
 
 val th7 = store_thm("th7", el 7 goals |> concl,
   rpt gen_tac
@@ -317,6 +327,7 @@ val th20 = store_thm("th20", el 20 goals |> concl,
   rpt gen_tac \\ MATCH_ACCEPT_TAC (CONJ (SPEC_ALL if_T) (SPEC_ALL if_F)))
 
 val forall_eq = hd(amatch``∀x. (x = t) ⇒ _``)
+val forall_eq2 = hd(amatch``∀x. (t = x) ⇒ _``)
 
 val ex_def = hd(amatch``$? = _``)
 val select_ax = hd(amatch ``p t ⇒ p ($@ p)``)
@@ -367,12 +378,6 @@ val th26 = store_thm("th26", el 26 goals |> concl,
 (* 27 TYPE_DEFINITION *)
 
 val not_T = hd(amatch``¬T``)
-
-val T_or = hd(amatch``T ∨ t``)
-val or_T = hd(amatch``t ∨ T``)
-val F_or = hd(amatch``F ∨ t``)
-val or_F = hd(amatch``t ∨ F``)
-val or_i = hd(amatch``t ∨ t``)
 
 val th28 = store_thm("th28", el 28 goals |> concl,
   rpt gen_tac
@@ -690,6 +695,162 @@ val th83 = store_thm("th83", el 83 goals |> concl,
   PURE_REWRITE_TAC[not_not]
   \\ strip_tac)
 
+val tc_def = hd(amatch``∀x. Relation_transitiveClosure x = _``)
+
+val bigIntersect_thm = hd(amatch``Relation_bigIntersect a b c ⇔ _``)
+
+val mem_fromPred = hd(amatch``Set_member r (Set_fromPredicate _)``)
+
+val subrelation_thm = hd(amatch``Relation_subrelation x s ⇔ ∀x y. _``)
+
+val transitive_thm = hd(amatch``Relation_transitive s ⇔ _``)
+
+val th84 = store_thm("th84", el 84 goals |> concl,
+  PURE_REWRITE_TAC[GSYM fun_eq_thm]
+  \\ PURE_REWRITE_TAC[tc_def,bigIntersect_thm,mem_fromPred]
+  \\ CONV_TAC(DEPTH_CONV BETA_CONV)
+  \\ Ho_Rewrite.PURE_REWRITE_TAC[ex_imp]
+  \\ PURE_REWRITE_TAC[subrelation_thm,transitive_thm]
+  \\ PURE_ONCE_REWRITE_TAC[GSYM and_imp_intro]
+  \\ Ho_Rewrite.PURE_REWRITE_TAC[forall_eq2]
+  \\ rpt gen_tac
+  \\ PURE_REWRITE_TAC[GSYM and_imp_intro]
+  \\ REFL_TAC)
+
+(* 85 TYPE_DEFINITION *)
+
+val wellFounded_thm = hd(amatch``Relation_wellFounded r ⇔ ∀p. (∃x. _) ⇒ _``)
+
+val th86 = store_thm("th86", el 86 goals |> concl,
+  PURE_REWRITE_TAC[GSYM fun_eq_thm]
+  \\ PURE_REWRITE_TAC[wellFounded_thm]
+  \\ CONV_TAC(DEPTH_CONV BETA_CONV)
+  \\ gen_tac \\ REFL_TAC)
+
+val less_thm = hd(amatch``Number_Natural_less _ _ ⇔ ∃x. _``)
+val less_refl = hd(amatch``Number_Natural_less x x``)
+val less_zero = hd(amatch``¬(Number_Natural_less _ (Number_Natural_zero))``)
+val less_suc_suc = hd(amatch``Number_Natural_less (Number_Natural_suc _) b``)
+
+val less_suc = hd(amatch``Number_Natural_less n (Number_Natural_suc n)``)
+val less_trans = hd(amatch``Number_Natural_less x y ∧ Number_Natural_less y z ⇒ _``)
+
+val num_cases = hd(amatch``(n = Number_Natural_zero) ∨ ∃n. _``)
+
+val num_ind = hd(amatch``_ ⇒ ∀n. P (n:Number_Natural_natural)``)
+
+val num_less_ind = hd(amatch``(∀x. _ ⇒ _) ⇒ ∀n. P (n:Number_Natural_natural)``)
+
+val not_less = hd(amatch``¬(Number_Natural_less _ _) ⇔ _``)
+
+val less_lesseq = hd(amatch``Number_Natural_less m (Number_Natural_suc n) ⇔  Number_Natural_lesseq m n``)
+
+val less_or_eq = hd(amatch``Number_Natural_lesseq _ _ ⇔ (Number_Natural_less _ _) ∨ _``)
+
+val trichotomy = hd(amatch``_ ∨ _ ∨ (_ = _)``)
+
+val th87 = store_thm("th87", el 87 goals |> concl,
+  PURE_REWRITE_TAC[GSYM fun_eq_thm]
+  \\ qx_genl_tac[`a`,`b`]
+  \\ CONV_TAC(DEPTH_CONV BETA_CONV)
+  \\ match_mp_tac (PURE_REWRITE_RULE[and_imp_intro]th23)
+  \\ conj_tac \\ strip_tac
+  >- (
+    qexists_tac`λx. Number_Natural_less x b`
+    \\ CONV_TAC(DEPTH_CONV BETA_CONV)
+    \\ reverse conj_tac
+    >- (
+      conj_tac >- (first_assum ACCEPT_TAC)
+      \\ MATCH_ACCEPT_TAC less_refl )
+    \\ gen_tac
+    \\ Q.ISPEC_THEN`b`FULL_STRUCT_CASES_TAC num_cases
+    >- (
+      PURE_REWRITE_TAC[EQF_INTRO (SPEC_ALL less_zero)]
+      \\ disch_then ACCEPT_TAC)
+    \\ PURE_REWRITE_TAC[less_suc_suc]
+    \\ strip_tac
+    \\ match_mp_tac less_trans
+    \\ qexists_tac`n'`
+    \\ conj_tac >- (first_assum ACCEPT_TAC)
+    \\ MATCH_ACCEPT_TAC less_suc )
+  \\ `∀n. Number_Natural_less n a ⇒ P n`
+  by (
+    qpat_assum`P a`mp_tac
+    \\ qid_spec_tac`a`
+    \\ ho_match_mp_tac num_ind
+    \\ conj_tac
+    >- (
+      PURE_REWRITE_TAC[EQF_INTRO (SPEC_ALL less_zero)]
+      \\ ntac 2 strip_tac
+      \\ CONV_TAC(REWR_CONV F_imp))
+    \\ rpt strip_tac
+    \\ `P a` by (first_x_assum(fn th => (first_x_assum match_mp_tac \\ first_assum ACCEPT_TAC)))
+    \\ `∀n. Number_Natural_less n a ⇒ P n` by (first_x_assum match_mp_tac \\ first_assum ACCEPT_TAC)
+    \\ first_x_assum(assume_tac o CONV_RULE(REWR_CONV less_lesseq))
+    \\ first_x_assum(strip_assume_tac o CONV_RULE(REWR_CONV less_or_eq))
+    >- (
+      first_x_assum match_mp_tac
+      \\ first_assum ACCEPT_TAC)
+    \\ VAR_EQ_TAC
+    \\ first_assum ACCEPT_TAC )
+  \\ qspecl_then[`a`,`b`]strip_assume_tac trichotomy
+  >- (
+    qspec_then`Number_Natural_less a b`(match_mp_tac o EQT_ELIM) F_imp
+    \\ qspec_then`¬(P b)`(match_mp_tac o UNDISCH) th50
+    \\ PURE_REWRITE_TAC[not_not]
+    \\ first_x_assum match_mp_tac
+    \\ first_assum ACCEPT_TAC )
+  \\ VAR_EQ_TAC
+  \\ first_x_assum(assume_tac o EQF_INTRO)
+  \\ first_x_assum(fn th => (first_x_assum(mp_tac o EQ_MP th)))
+  \\ PURE_REWRITE_TAC[F_imp])
+
+val th88 = store_thm("th88", el 88 goals |> concl,
+  PURE_REWRITE_TAC[GSYM fun_eq_thm,transitive_thm]
+  \\ CONV_TAC(DEPTH_CONV BETA_CONV)
+  \\ gen_tac \\ REFL_TAC)
+
+val th89 = store_thm("th89", el 89 goals |> concl,
+  PURE_REWRITE_TAC[GSYM fun_eq_thm,subrelation_thm]
+  \\ CONV_TAC(DEPTH_CONV BETA_CONV)
+  \\ rpt gen_tac \\ REFL_TAC)
+
+(* 90 - pre is more specified in HOL than in OT *)
+
+val union_thm = hd(amatch``Relation_union r s = _``)
+val fromSet_thm = hd(amatch``Relation_fromSet _ _ _``)
+val mem_union = hd(amatch``Set_member _ (Set_union _ _) ⇔ _``)
+val mem_toSet = hd(amatch``Set_member _ (Relation_toSet _)``)
+
+val th91 = store_thm("th91", el 91 goals |> concl,
+  PURE_REWRITE_TAC[GSYM fun_eq_thm,union_thm,fromSet_thm,mem_union,mem_toSet]
+  \\ CONV_TAC(DEPTH_CONV BETA_CONV)
+  \\ rpt gen_tac \\ REFL_TAC)
+
+val intersect_thm = hd(amatch``Relation_intersect x y = _``)
+
+val mem_inter = hd(amatch``Set_member _ (Set_intersect _ _)``)
+
+val th92 = store_thm("th92", el 92 goals |> concl,
+  PURE_REWRITE_TAC[GSYM fun_eq_thm,intersect_thm,fromSet_thm,mem_inter,mem_toSet]
+  \\ CONV_TAC(DEPTH_CONV BETA_CONV)
+  \\ rpt gen_tac \\ REFL_TAC)
+
+val greatereq_thm = hd(amatch``Number_Natural_greatereq _ _``)
+val greater_thm = hd(amatch``Number_Natural_greater _ _ = _``)
+
+val th93 = store_thm("th93", el 93 goals |> concl,
+  PURE_REWRITE_TAC[GSYM fun_eq_thm,greatereq_thm,less_or_eq,greater_thm]
+  \\ CONV_TAC(DEPTH_CONV BETA_CONV)
+  \\ rpt gen_tac
+  \\ CONV_TAC(RAND_CONV(ONCE_DEPTH_CONV SYM_CONV))
+  \\ REFL_TAC)
+
+val th94 = store_thm("th94", el 94 goals |> concl,
+  PURE_REWRITE_TAC[GSYM fun_eq_thm,less_or_eq]
+  \\ CONV_TAC(DEPTH_CONV BETA_CONV)
+  \\ rpt gen_tac \\ REFL_TAC)
+
 val th95 = store_thm("th95", el 95 goals |> concl,
   MATCH_ACCEPT_TAC ex_unique_thm)
 
@@ -754,6 +915,110 @@ val th105 = store_thm("th105", el 105 goals |> concl,
 val left_11 = hd(amatch``Data_Sum_left _ = Data_Sum_left _``)
 val th106 = store_thm("th106", el 106 goals |> concl,
   MATCH_ACCEPT_TAC left_11)
+
+val min_thm = hd(amatch``Number_Natural_min _ _ = COND _ _ _``)
+
+val if_id = hd(amatch``if _ then x else x``)
+
+val th107 = store_thm("th107", el 107 goals |> concl,
+  PURE_REWRITE_TAC[GSYM fun_eq_thm,min_thm,less_or_eq]
+  \\ CONV_TAC(DEPTH_CONV BETA_CONV)
+  \\ rpt gen_tac
+  \\ qspec_then`x = x'`strip_assume_tac bool_cases
+  \\ first_assum SUBST1_TAC
+  \\ PURE_REWRITE_TAC[or_F,or_T,if_T]
+  \\ TRY REFL_TAC
+  \\ pop_assum(SUBST1_TAC o EQT_ELIM)
+  \\ PURE_REWRITE_TAC[if_id]
+  \\ REFL_TAC)
+
+val max_thm = hd(amatch``Number_Natural_max _ _ = COND _ _ _``)
+
+val th108 = store_thm("th108", el 108 goals |> concl,
+  PURE_REWRITE_TAC[GSYM fun_eq_thm,max_thm,less_or_eq]
+  \\ CONV_TAC(DEPTH_CONV BETA_CONV)
+  \\ rpt gen_tac
+  \\ qspec_then`x = x'`strip_assume_tac bool_cases
+  \\ first_assum SUBST1_TAC
+  \\ PURE_REWRITE_TAC[or_F,or_T,if_T]
+  \\ TRY REFL_TAC
+  \\ pop_assum(SUBST1_TAC o EQT_ELIM)
+  \\ PURE_REWRITE_TAC[if_id]
+  \\ REFL_TAC)
+
+val bit1_thm = hd(amatch``Number_Natural_bit1 _ = _``)
+val bit0_suc = hd(amatch``Number_Natural_bit0 _ = _ _``)
+val bit0_zero = hd(amatch``Number_Natural_bit0 Number_Natural_zero``)
+val plus_zero = hd(amatch``Number_Natural_plus Number_Natural_zero _``)
+val plus_suc = hd(amatch``Number_Natural_plus _ (Number_Natural_suc _)``)
+val plus_suc1 = hd(amatch``Number_Natural_plus (Number_Natural_suc _) _``)
+
+val th109 = store_thm("th109", el 109 goals |> concl,
+  PURE_REWRITE_TAC[GSYM fun_eq_thm,bit1_thm,plus_suc]
+  \\ CONV_TAC(DEPTH_CONV BETA_CONV)
+  \\ gen_tac
+  \\ AP_TERM_TAC
+  \\ qid_spec_tac`x`
+  \\ ho_match_mp_tac num_ind
+  \\ PURE_REWRITE_TAC[bit0_zero,bit0_suc,plus_zero,plus_suc1]
+  \\ conj_tac >- REFL_TAC
+  \\ gen_tac
+  \\ disch_then SUBST_ALL_TAC
+  \\ PURE_REWRITE_TAC[plus_suc]
+  \\ REFL_TAC)
+
+val irreflexive_thm = hd(amatch``Relation_irreflexive _ = _``)
+
+val th110 = store_thm("th110", el 110 goals |> concl,
+  PURE_REWRITE_TAC[GSYM fun_eq_thm, irreflexive_thm]
+  \\ CONV_TAC (DEPTH_CONV BETA_CONV)
+  \\ rpt gen_tac
+  \\ REFL_TAC)
+
+val reflexive_thm = hd(amatch``Relation_reflexive _ = _``)
+
+val th111 = store_thm("th111", el 111 goals |> concl,
+  PURE_REWRITE_TAC[GSYM fun_eq_thm, reflexive_thm]
+  \\ CONV_TAC (DEPTH_CONV BETA_CONV)
+  \\ rpt gen_tac \\ REFL_TAC)
+
+val o_thm = hd(amatch``(Function_o _ _) _ = _``)
+
+val th112 = store_thm("th112", el 112 goals |> concl,
+  PURE_REWRITE_TAC[GSYM fun_eq_thm,o_thm]
+  \\ CONV_TAC (DEPTH_CONV BETA_CONV)
+  \\ rpt gen_tac \\ REFL_TAC)
+
+val th113 = store_thm("th113", el 113 goals |> concl,
+  PURE_REWRITE_TAC[GSYM fun_eq_thm,greater_thm]
+  \\ CONV_TAC (DEPTH_CONV BETA_CONV)
+  \\ rpt gen_tac \\ REFL_TAC)
+
+(* 114, 115 - LET, IN *)
+
+val skk = hd(amatch``Function_Combinator_s _ _ = Function_id``)
+
+val th116 = store_thm("th116", el 116 goals |> concl,
+  PURE_REWRITE_TAC[skk] \\ REFL_TAC)
+
+val one_thm = hd(amatch``_ = Data_Unit_unit``)
+
+val th117 = store_thm("th117", el 117 goals |> concl,
+  PURE_ONCE_REWRITE_TAC[one_thm] \\ REFL_TAC)
+
+val universe_thm = hd(amatch``Relation_universe _ _``)
+
+val th118 = store_thm("th118", el 118 goals |> concl,
+  PURE_REWRITE_TAC[GSYM fun_eq_thm,EQT_INTRO(SPEC_ALL universe_thm)]
+  \\ CONV_TAC (DEPTH_CONV BETA_CONV)
+  \\ rpt gen_tac \\ REFL_TAC)
+
+val empty_thm = hd(amatch``Relation_empty _ _``)
+
+val th119 = store_thm("th119", el 119 goals |> concl,
+  PURE_REWRITE_TAC[GSYM fun_eq_thm,EQF_INTRO (SPEC_ALL empty_thm)]
+  \\ CONV_TAC (DEPTH_CONV BETA_CONV)
+  \\ rpt gen_tac \\ REFL_TAC)
 
 val th120 = store_thm("th120", el 120 goals |> concl,
   REFL_TAC)
